CollapsingTowers/TwoLevelMut/LogicalEquiv/Compatibility.lean
@@ -1,0 +1,21 @@
+import CollapsingTowers.TwoLevelMut.LogicalEquiv.LogicalRelation
+
+-- Γ ⊧ x ≈𝑙𝑜𝑔 x : Γ(x)
+lemma compatibility.fvar :
+  ∀ Γ x τ,
+    binds x (τ, 𝟚) Γ →
+    wbt 𝟚 τ →
+    log_equiv Γ (.fvar x) (.fvar x) τ :=
+  by
+  intros Γ x τ Hbinds Hwbt
+  constructor; apply typing.fvar; apply Hbinds; apply Hwbt
+  constructor; apply typing.fvar; apply Hbinds; apply Hwbt
+  intros 𝓦 γ₀ γ₁ HsemΓ
+  simp only [log_equiv_expr]
+  intros σ₀ σ₁ Hsem_store
+  exists 𝓦, σ₀, σ₁, msubst γ₀ (.fvar x), msubst γ₁ (.fvar x)
+  constructor; admit
+  constructor; apply stepn.refl
+  constructor; apply stepn.refl
+  constructor; apply Hsem_store
+  admit
