CollapsingTowers/TwoLevelMut/LogicalEquiv/Defs.lean
@@ -1,1 +1,3 @@
+import CollapsingTowers.TwoLevelMut.LogicalEquiv.World
 import CollapsingTowers.TwoLevelMut.LogicalEquiv.LogicalRelation
+import CollapsingTowers.TwoLevelMut.LogicalEquiv.Compatibility
