CollapsingTowers/TwoLevelMut/LogicalEquiv/World.lean
@@ -1,0 +1,23 @@
+import Mathlib.Data.Nat.Basic
+
+@[simp]
+def bijection {α β} (r : α → β → Prop): Prop :=
+  (∀ x y z, r x y → r x z → y = z) ∧
+  (∀ x y z, r x z → r y z → x = y)
+
+abbrev World :=
+  ℕ → ℕ → Prop
+
+@[simp]
+def World.future (𝓦₀ 𝓦₁ : World) : Prop :=
+  ∀ x y, 𝓦₁ x y → 𝓦₀ x y
+
+notation:max 𝓦₁ " ⊒ " 𝓦₀  => World.future 𝓦₀ 𝓦₁
+
+@[simp]
+def World.empty : World :=
+  fun _ _ => false
+
+@[simp]
+def World.ext (𝓦 : World) (l₀ l₁ : ℕ) : World :=
+  fun x y => (x = l₀ ∧ y = l₁) ∨ 𝓦 l₀ l₁
